wip

Foundation/Modal/Kripke/SimpleExtension.lean
@@ -81,6 +81,8 @@ namespace Model.extendRoot
 
 variable {M : Model} {r : M.World} [M.IsRooted r] {x y : M.World}
 
+protected abbrev root := Frame.extendRoot.root (F := M.toFrame) (r := r)
+
 def pMorphism : Model.PseudoEpimorphism M (M.extendRoot r) := Model.PseudoEpimorphism.ofAtomic (@Frame.extendRoot.pMorphism M.toFrame r inferInstance) $ by
   intros; rfl;
 
