Foundation/Modal/Kripke/Hilbert/GL/Unnecessitation.lean
@@ -9,35 +9,43 @@ open Formula.Kripke
 
 namespace Hilbert.GL
 
+open Model in
 lemma imply_boxdot_plain_of_imply_box_box : Hilbert.GL ⊢! □φ ➝ □ψ → Hilbert.GL ⊢! ⊡φ ➝ ψ := by
   contrapose;
   intro h;
   have := Kripke.iff_unprovable_exists_unsatisfies_FiniteTransitiveTree.mp h;
-  obtain ⟨M, hs⟩ := this;
+  obtain ⟨M, r, M_tree, hs⟩ := this;
 
-  have hs : Satisfies M.toModel M.root (⊡φ ⋏ ∼ψ) := by simp_all [Satisfies, Semantics.Realize];
-  replace hs := @FiniteTransitiveTreeModel.SimpleExtension.modal_equivalence_original_world M M.root (⊡φ ⋏ ∼ψ) |>.mp hs;
+  have hs : Satisfies M r (⊡φ ⋏ ∼ψ) := by simp_all [Satisfies, Semantics.Realize];
+  have := @Model.extendRoot.modal_equivalence_original_world (M := M) (r := r) inferInstance r (⊡φ ⋏ ∼ψ) |>.mp hs;
   have ⟨hs₁₂, hs₃⟩ := Satisfies.and_def.mp hs;
   have ⟨hs₁, hs₂⟩ := Satisfies.and_def.mp hs₁₂;
 
-  have hbp : Satisfies M↧.toModel (M↧.root) (□φ) := by
+  let M₀ := M.extendRoot r;
+  let r₀ : M₀.World := extendRoot.root (r := r)
+
+  have hbp : Satisfies M₀ r₀ (□φ) := by
     intro x hx;
-    rcases @Kripke.FiniteTransitiveTree.SimpleExtension.through_original_root M.toFiniteTransitiveTree x hx with (rfl | hr);
-    . assumption;
-    . apply hs₂;
-      exact hr;
-  have hbq : ¬(Satisfies M↧.toModel (M↧.root) (□ψ)) := by
+    rcases Frame.extendRoot.through_original_root (F := M.toFrame) (x := x) hx with (rfl | hr);
+    . sorry;
+      -- assumption;
+    . sorry;
+      -- apply hs₂;
+      -- exact hr;
+  have hbq : ¬(Satisfies M₀ r₀ (□ψ)) := by
     apply Satisfies.box_def.not.mpr;
     push_neg;
-    use M.root;
+    use (Sum.inr r);
     constructor;
-    . apply M↧.toRootedFrame.root_rooted M.root;
-      simp [FiniteTransitiveTreeModel.SimpleExtension, Kripke.FiniteTransitiveTree.SimpleExtension]; -- TODO: extract lemma
-    . assumption;
+    . sorry;
+      -- apply M↧.toRootedFrame.root_rooted M.root;
+      -- simp [FiniteTransitiveTreeModel.SimpleExtension, Kripke.FiniteTransitiveTree.SimpleExtension]; -- TODO: extract lemma
+    . sorry;
+      -- assumption;
 
   apply Kripke.iff_unprovable_exists_unsatisfies_FiniteTransitiveTree.mpr;
-  use M↧;
-  exact _root_.not_imp.mpr ⟨hbp, hbq⟩;
+  use M₀, r₀;
+  tauto;
 
 theorem unnecessitation! : Hilbert.GL ⊢! □φ → Hilbert.GL ⊢! φ := by
   intro h;
